Change of contracted session type representation
Contracted session types now carry a non-empty list of variables in mu
binders rather than a set. This ensures that the conversion from regular
to contracted session types is reversible; this property is proven in
Conv.v. Note, however, that the conversion in the opposite direction is
not reversible if the source type has a component of the form

  mu [X1, ..., Xn]. mu [Y1, ..., Ym]. S

This change of representation necessitates the reformulation of a bunch
of related theorems.

Conv.v also currently has a proof for

  wellformed S -> wellformed (conv S)

where S is a regular session type and (conv S) is the corresponding
contracted session type.

In order for the conversion to become useful, we still need

  S ~ T <-> (conv S) ~' (conv T)

where ~ and ~' denote equivalence.

Conv.v
@@ -1,41 +1,43 @@
-Require Import Env Morphisms Msg SessionTypes SessionTypesC Shape Var
-  Wellformed WellformedC.
+Require Import Arith.Lt Env List ListAux List1 Logic.FunctionalExtensionality
+  Morphisms Msg Program.Equality SessionTypes SessionTypesC Shape TLC.LibTactics
+  Var Vars Wellformed WellformedC.
+Import ListNotations.
 
 Module R := Sty.
 Module C := StyC.
 
-Fixpoint sty_styC_aux (xs : Env) (S : R.Sty) : C.Sty :=
+Fixpoint sty_styC_aux (xs : list Var) (S : R.Sty) : C.Sty :=
   match S with
   | R.unit => C.unit
-  | R.send B S' => C.send B (sty_styC_aux env_empty S')
-  | R.recv B S' => C.recv B (sty_styC_aux env_empty S')
-  | R.echoice S1 S2 => C.echoice (sty_styC_aux env_empty S1) (sty_styC_aux env_empty S2)
-  | R.ichoice S1 S2 => C.ichoice (sty_styC_aux env_empty S1) (sty_styC_aux env_empty S2)
+  | R.send B S' => C.send B (sty_styC_aux [] S')
+  | R.recv B S' => C.recv B (sty_styC_aux [] S')
+  | R.echoice S1 S2 => C.echoice (sty_styC_aux [] S1) (sty_styC_aux [] S2)
+  | R.ichoice S1 S2 => C.ichoice (sty_styC_aux [] S1) (sty_styC_aux [] S2)
   | R.mu x S' =>
     match S' with
-    | R.mu _ _ => sty_styC_aux (env_add x xs) S'
-    | _        => C.mu (env_add x xs) (sty_styC_aux env_empty S')
+    | R.mu _ _ => sty_styC_aux (x :: xs) S' (* [Note rev-variable-order] *)
+    | _        => C.mu (list_to_list1 x xs) (sty_styC_aux [] S')
     end
   | R.var X => C.var X
   end
 .
 Arguments sty_styC_aux xs S : simpl nomatch.
 
-Instance sty_styC_aux_m : Proper (env_eq ==> eq ==> C.eq_syn) sty_styC_aux.
-Proof.
-  unfold Proper. unfold respectful. intros e e' Hee' x y Hxy. subst.
-  rename y into S. generalize dependent e'. generalize dependent e.
-  induction S; intros e e' Hee'; simpl in *; try solve
-    [ constructor; auto; first [apply IHS | apply IHS1 | apply IHS2]
-    ; reflexivity
-    ].
+(* [Note rev-variable-order]
+Note that the variable ordering is reversed here: The regular session type
 
-    destruct S; simpl in *; try solve
-      [constructor; [rewrite Hee'; reflexivity | eauto]].
-      eapply IHS. rewrite Hee'. reflexivity.
-Qed.
+  mu X. mu Y. S
 
-Notation sty_styC := (sty_styC_aux env_empty).
+becomes the contracted session type
+
+  mu [Y, X]. S
+
+This makes no difference semantically since variable ordering in a chain of
+binders is irrelevant, but it's easier to define. We'll see if the proofs
+become more difficult as a result.
+*)
+
+Notation sty_styC := (sty_styC_aux []).
 
 Fixpoint styC_sty (S : C.Sty) : R.Sty :=
   match S with
@@ -44,135 +46,252 @@ Fixpoint styC_sty (S : C.Sty) : R.Sty :=
   | C.recv B S' => R.recv B (styC_sty S')
   | C.echoice S1 S2 => R.echoice (styC_sty S1) (styC_sty S2)
   | C.ichoice S1 S2 => R.ichoice (styC_sty S1) (styC_sty S2)
-  | C.mu xs S' => env_fold (fun X S'' => R.mu X S'') xs (styC_sty S')
+  | C.mu xs S' => fold_left1 (fun S X => R.mu X S) xs (styC_sty S')
+    (* [Note fold-left-not-right] *)
   | C.var X => R.var X
   end
 .
 
+(* [Note fold-left-not-right]
+The left fold reverses the variable ordering again to make sty_styC and
+styC_sty inverses of each other.
+*)
+
+Section Inverses.
+
+(* TODO beautify *)
+Lemma styC_sty_inverse_sty_styC_aux :
+  forall S,
+  (R.shape S <> muS ->
+    forall xs, styC_sty (sty_styC_aux xs S) = S) /\
+  (R.shape S = muS ->
+    styC_sty (sty_styC_aux [] S) = S /\
+    forall x xs,
+    styC_sty (sty_styC_aux (xs ++ [x]) S) =
+    R.mu x (styC_sty (sty_styC_aux xs S))).
+Proof.
+  induction S; split; introv Hshape; try discriminate; intros.
+    simpl. trivial.
+
+    simpl in *. destruct IHS as [IHSnomu IHSmu].
+    destruct (R.shape_dec S muS) as [HSmu | HSnomu].
+      apply IHSmu in HSmu. destruct HSmu as [H _]. rewrite H. trivial.
+      rewrite IHSnomu; auto.
+
+    simpl in *. destruct IHS as [IHSnomu IHSmu].
+    destruct (R.shape_dec S muS) as [HSmu | HSnomu].
+      apply IHSmu in HSmu. destruct HSmu as [H _]. rewrite H. trivial.
+      rewrite IHSnomu; auto.
+
+    simpl in *.
+    destruct IHS1 as [IHS1nomu IHS1mu]. destruct IHS2 as [IHS2nomu IHS2mu].
+      destruct (R.shape_dec S1 muS) as [HS1mu | HS1nomu];
+      destruct (R.shape_dec S2 muS) as [HS2mu | HS2nomu].
+        apply IHS1mu in HS1mu. destruct HS1mu as [H1 _]. rewrite H1.
+        apply IHS2mu in HS2mu. destruct HS2mu as [H2 _]. rewrite H2.
+        trivial.
+
+        apply IHS1mu in HS1mu. destruct HS1mu as [H1 _]. rewrite H1.
+        rewrite IHS2nomu; auto.
+
+        rewrite IHS1nomu; auto.
+        apply IHS2mu in HS2mu. destruct HS2mu as [H2 _]. rewrite H2. trivial.
+
+        rewrite IHS1nomu; auto.
+        rewrite IHS2nomu; auto.
+
+    simpl in *.
+    destruct IHS1 as [IHS1nomu IHS1mu]. destruct IHS2 as [IHS2nomu IHS2mu].
+      destruct (R.shape_dec S1 muS) as [HS1mu | HS1nomu];
+      destruct (R.shape_dec S2 muS) as [HS2mu | HS2nomu].
+        apply IHS1mu in HS1mu. destruct HS1mu as [H1 _]. rewrite H1.
+        apply IHS2mu in HS2mu. destruct HS2mu as [H2 _]. rewrite H2.
+        trivial.
+
+        apply IHS1mu in HS1mu. destruct HS1mu as [H1 _]. rewrite H1.
+        rewrite IHS2nomu; auto.
+
+        rewrite IHS1nomu; auto.
+        apply IHS2mu in HS2mu. destruct HS2mu as [H2 _]. rewrite H2. trivial.
+
+        rewrite IHS1nomu; auto.
+        rewrite IHS2nomu; auto.
+
+    unfold not in Hshape. exfalso. auto.
+
+    destruct IHS as [IHSnomu IHSmu]. split.
+      destruct S; simpl in *; try solve
+        [trivial | rewrite IHSnomu; unfold not; try discriminate; auto; constructor].
+
+        destruct IHSmu. auto. specialize H0 with (x := v) (xs := nil).
+        simpl in H0. rewrite H in H0. assumption.
+
+     intros. gen x. destruct S; intros; try solve
+       [simpl; rewrite fold_left_snoc; trivial].
+
+       destruct IHSmu. auto. simpl. specialize H0 with (x := x) (xs := (v :: xs)).
+       assumption.
+
+    auto.
+Qed.
+
+Lemma styC_sty_inverse_sty_styC :
+  forall S,
+  styC_sty (sty_styC S) = S.
+Proof.
+  intros. remember styC_sty_inverse_sty_styC_aux as H.
+  edestruct H as [Hnomu Hmu]. destruct (R.shape_dec S muS);
+    [apply Hmu | apply Hnomu]; auto.
+Qed.
+
+End Inverses.
+
 Section Wf.
 
-(* TODO beautify *)
+Lemma sty_styC_aux_ok_assoc :
+  forall S e xs ys x y,
+  WfC.ok e (sty_styC_aux (xs ++ x :: y :: ys) S) ->
+  WfC.ok e (sty_styC_aux (xs ++ y :: x :: ys) S).
+Proof.
+  assert (
+    forall e v xs x y ys HxsNE,
+    env_eq (env_union_vars e (mkList1 (v :: xs ++ x :: y :: ys) HxsNE))
+           (env_union_vars e (mkList1 (v :: xs ++ y :: x :: ys)
+                               (cons_not_nil Var v (xs ++ y :: x :: ys))))
+  ) as Hcomm.
+    intros. repeat (rewrite env_union_vars_spec). simpl.
+    asserts_rewrite (env_eq (list_to_env (xs ++ x :: y :: ys))
+                            (list_to_env (xs ++ y :: x :: ys))).
+      unfold env_eq. intro. repeat (rewrite SF.of_list_1).
+      repeat (rewrite SetoidList.InA_app_iff); auto with typeclass_instances.
+      repeat (rewrite SetoidList.InA_cons); auto with typeclass_instances.
+      iauto.
+    reflexivity.
+  induction S; introv H; try solve [simpl; constructor; inverts H; auto].
+    destruct S; simpl in *; try solve
+      [ simpl in *; constructor; unfold not; try discriminate
+      ; solve [constructor | inverts H; rewrite Hcomm; auto ]
+      ].
+
+      simpl in *. specialize IHS with (e := e) (xs := v :: xs). apply IHS.
+      auto.
+
+      inverts H. contradict H2. auto.
+Qed.
+
+Lemma sty_styC_aux_ok_assoc' :
+  forall S e x y zs,
+  WfC.ok e (sty_styC_aux (x :: y :: zs) S) ->
+  WfC.ok e (sty_styC_aux (y :: x :: zs) S).
+Proof.
+  introv H. asserts_rewrite (y :: x :: zs = [] ++ y :: x :: zs). auto.
+  apply sty_styC_aux_ok_assoc. auto.
+Qed.
+
+Lemma sty_styC_aux_ok_expansion :
+  forall S e e' X,
+  R.shape S = muS ->
+  WfC.ok (env_add X e) (sty_styC_aux e' S) ->
+  WfC.ok e (sty_styC_aux (X :: e') S).
+Proof.
+  assert (
+    forall X e v e',
+    env_eq (env_union_vars (env_add X e) (mkList1 (v :: e') (cons_not_nil Var v e')))
+           (env_union_vars e (mkList1 (v :: X :: e') (cons_not_nil Var v (X :: e'))))
+  ) as Heq.
+    intros. repeat (rewrite env_union_vars_spec). simpl.
+    rewrite env_union_add. rewrite env_add_assoc. reflexivity.
+
+  induction S; introv Hsh H; try discriminate.
+    destruct S; try solve
+      [ simpl in *; constructor; unfold not; try discriminate
+      ; first [solve [constructor] | inverts H; rewrite <- Heq; auto]
+      ].
+
+      simpl in *. apply sty_styC_aux_ok_assoc'. apply IHS; auto.
+
+      simpl in *. inverts H. exfalso. auto.
+Qed.
+
+(* TODO extract the "unfold not; discriminate" dance into a tactic ("ineq"?) *)
+(* TODO why is "auto with wf" not working? *)
+Lemma sty_styC_aux_checked :
+  forall S e e',
+  Wf.checked e S ->
+  WfC.ok e (sty_styC_aux e' S).
+Proof.
+  assert (
+    forall v e e',
+    env_subset (env_add v e)
+               (env_union_vars e (mkList1 (v :: e') (cons_not_nil Var v e')))
+  ) as Hsub.
+    intros. rewrite env_union_vars_spec. unfold SF.of_list. simpl.
+    rewrite <- env_add_union2. apply env_add_m_subset. auto with set.
+  induction S; introv H; try solve
+    [ auto with wf
+    | simpl; do 2 (inverts H as H); asserts_rewrite (e = env_union_list e [])
+    ; auto with wf
+    ].
+
+    destruct S; simpl in *;
+      try solve
+        [ constructor; unfold not; try discriminate; do 3 (inverts H as H)
+        ; apply IHS; auto; rewrite <- Hsub; constructor; constructor; auto
+        ].
+
+      do 3 (inverts H as H). apply sty_styC_aux_ok_expansion; [auto | idtac].
+      apply IHS. constructor. constructor. auto.
+
+    simpl. constructor. inverts H as H; [auto | inverts H].
+Qed.
+
 Lemma sty_styC_aux_ok :
-  forall S e e' e'',
-  WfC.ok e (sty_styC_aux (env_union e' e'') S) ->
-  (R.shape S = muS -> WfC.ok (env_union e e') (sty_styC_aux e''       S)) /\
-  (R.shape S <> muS -> WfC.ok e               (sty_styC_aux env_empty S)).
+  forall S e e',
+  Wf.ok e S ->
+  WfC.ok (env_union_list e e') (sty_styC_aux e' S).
 Proof.
-  induction S; intros e e' e'' H; simpl in *; split; intro HsS;
-    try (discriminate || auto).
+  assert (
+    forall v e e',
+    env_subset (env_union_list (env_add v e) e')
+               (env_union_vars (env_union_list e e')
+                 (mkList1 (v :: e') (cons_not_nil Var v e')))
+  ) as Hsub.
+    intros. rewrite env_union_vars_spec. rewrite env_union_list_spec.
+    simpl. rewrite <- env_add_union2. rewrite env_add_union1.
+    apply SF.union_subset_4. rewrite env_union_list_spec. (* TODO *)
+    apply env_add_m_subset. apply env_subset_union1.
+  (* TODO move to Env.v? *)
+  assert (
+    forall e e',
+    env_subset (env_union_list e []) (env_union_list e e')
+  ) as Hsub'.
+    intros. repeat (rewrite env_union_list_spec). simpl.
+    rewrite env_union_neutral. apply env_subset_union1.
+  induction S; introv H; try solve
+    [ simpl; constructor; inverts H; rewrite <- Hsub'; simpl
+    ; apply sty_styC_aux_checked; auto
+    ].
 
-    destruct S; simpl in *.
-      constructor; unfold not; try discriminate. constructor.
+    destruct S; try solve
+      [ simpl in *; constructor; unfold not; try discriminate; auto
+      ; inverts H; rewrite <- Hsub; auto
+      ].
 
-      constructor; unfold not; try discriminate;
-      apply IHS; unfold not; auto; try discriminate;
-      inversion_clear H; rewrite env_union_assoc; rewrite <- env_add_union2; assumption.
+      simpl in *. apply sty_styC_aux_ok_expansion; [auto | idtac].
+      rewrite env_union_list_spec. rewrite env_add_union1.
+      rewrite <- env_union_list_spec. apply IHS. inverts H. assumption.
 
-      constructor; unfold not; try discriminate;
-      apply IHS; unfold not; auto; try discriminate;
-      inversion_clear H; rewrite env_union_assoc; rewrite <- env_add_union2; assumption.
-
-      constructor; unfold not; try discriminate;
-      apply IHS; unfold not; auto; try discriminate;
-      inversion_clear H; rewrite env_union_assoc; rewrite <- env_add_union2; assumption.
-
-      constructor; unfold not; try discriminate;
-      apply IHS; unfold not; auto; try discriminate;
-      inversion_clear H; rewrite env_union_assoc; rewrite <- env_add_union2; assumption.
-
-      apply IHS; auto. rewrite <- env_add_union2. assumption.
-
-      inversion_clear H. exfalso; unfold not; eapply H0; eauto.
-
-    unfold not in *; exfalso; apply HsS; trivial.
+      inverts H as H. inverts H.
 Qed.
+Hint Resolve sty_styC_aux_ok : wf.
 
-Lemma sty_styC_aux_mu :
-  forall S X e e',
-  WfC.ok e (sty_styC_aux e' (R.mu X S)) ->
-  WfC.ok (env_union e e') (sty_styC (R.mu X S)).
-Proof with auto.
-  intros. apply sty_styC_aux_ok... rewrite env_union_neutral...
-Qed.
-
-(* TODO beautify *)
-Lemma sty_styC_ok_checked :
-  forall S e,
-  WfC.ok e (sty_styC S) ->
-  (Wf.checked e S /\
-   ((forall X, S <> R.var X) ->
-    Wf.ok e S)
-  ).
-Proof with (auto with wf).
-  induction S; intros e H; split; intros.
-    constructor. constructor.
-    constructor.
-    constructor. constructor. inversion_clear H. edestruct IHS; eauto.
-    constructor. inversion_clear H. edestruct IHS; eauto.
-    constructor. constructor. inversion_clear H. edestruct IHS; eauto.
-    constructor. inversion_clear H. edestruct IHS; eauto.
-    constructor; constructor; inversion_clear H; [edestruct IHS1 | edestruct IHS2]; eauto.
-    constructor; inversion_clear H; [edestruct IHS1 | edestruct IHS2]; eauto.
-    constructor; constructor; inversion_clear H; [edestruct IHS1 | edestruct IHS2]; eauto.
-    constructor; inversion_clear H; [edestruct IHS1 | edestruct IHS2]; eauto.
-
-    destruct S; simpl in *.
-      constructor. constructor. constructor.
-
-      constructor. constructor. inversion_clear H. rewrite <- env_add_union_singleton.
-      edestruct IHS; eauto. eapply H3. unfold not. discriminate.
-
-      constructor. constructor. inversion_clear H. rewrite <- env_add_union_singleton.
-      edestruct IHS; eauto. eapply H3. unfold not. discriminate.
-
-      constructor; constructor; inversion_clear H; rewrite <- env_add_union_singleton;
-      edestruct IHS; eauto; eapply H3; unfold not; discriminate.
-
-      constructor; constructor; inversion_clear H; rewrite <- env_add_union_singleton;
-      edestruct IHS; eauto; eapply H3; unfold not; discriminate.
-
-      destruct IHS with (e := env_add v e); eauto.
-        rewrite <- env_add_union_singleton. apply sty_styC_aux_mu. assumption.
-      constructor. constructor. eapply H1. unfold not; discriminate.
-
-      constructor. constructor. inversion_clear H. edestruct IHS. eauto.
-      rewrite <- env_add_union_singleton. eapply H3. unfold not in *; intros.
-      eapply H0. eexists.
-
-    destruct S; simpl in *.
-      constructor. constructor.
-
-      constructor. inversion_clear H. edestruct IHS; eauto.
-      rewrite <- env_add_union_singleton. eapply H4. unfold not; discriminate.
-
-      constructor. inversion_clear H. edestruct IHS; eauto.
-      rewrite <- env_add_union_singleton. eapply H4. unfold not; discriminate.
-
-      constructor; inversion_clear H; edestruct IHS; eauto;
-      rewrite <- env_add_union_singleton; eapply H4; unfold not; discriminate.
-
-      constructor; inversion_clear H; edestruct IHS; eauto;
-      rewrite <- env_add_union_singleton; eapply H4; unfold not; discriminate.
-
-      constructor. destruct IHS with (e := env_add v e).
-        rewrite <- env_add_union_singleton. apply sty_styC_aux_mu. assumption.
-      eapply H2. unfold not; discriminate.
-
-      inversion_clear H. unfold not in *. exfalso. eapply H1. eexists.
-
-    inversion_clear H. constructor...
-
-    unfold not in *; exfalso; eauto.
-Qed.
-
-Lemma sty_styC_wf :
-  forall S,
-  WfC.wellformed (sty_styC S) ->
-  Wf.wellformed S.
+Lemma sty_styC_ok :
+  forall e S,
+  Wf.ok e S ->
+  WfC.ok e (sty_styC S).
 Proof.
-  intros. apply sty_styC_ok_checked; auto.
-    unfold not; intros; destruct S; inversion_clear H; try discriminate.
-    contradict H1. apply env_mem_empty.
+  introv H. rewrite <- env_union_list_neutral with (xs := e). auto with wf.
 Qed.
+Hint Resolve sty_styC_ok : wf.
 
 End Wf.
