SessionTypesC.v
@@ -1,5 +1,5 @@
 Require Import Env List List1 Morphisms Msg Relations.Relation_Definitions
-  Relations.Relation_Operators Shape Var.
+  Relations.Relation_Operators Shape Var Vars.
 Require Setoid.
 
 Create HintDb styc discriminated.
@@ -12,7 +12,7 @@ Inductive Sty : Type :=
 | recv : Msg -> Sty -> Sty
 | echoice : Sty -> Sty -> Sty
 | ichoice : Sty -> Sty -> Sty
-| mu : Env -> Sty -> Sty
+| mu : Vars -> Sty -> Sty
 | var : Var -> Sty
 .
 
@@ -23,7 +23,7 @@ Fixpoint subst (x : Var) (r orig : Sty) : Sty :=
   | recv msg tail => recv msg (subst x r tail)
   | echoice tail1 tail2 => echoice (subst x r tail1) (subst x r tail2)
   | ichoice tail1 tail2 => ichoice (subst x r tail1) (subst x r tail2)
-  | mu ys tail => if env_memb x ys then orig else mu ys (subst x r tail)
+  | mu ys tail => if In_Vars_dec x ys then orig else mu ys (subst x r tail)
   | var y => if beq_var x y then r else orig
   end
 .
@@ -39,69 +39,5 @@ Definition shape (S : Sty) : Shape :=
   | var _ => varS
   end
 .
-
-Inductive eq_syn : Sty -> Sty -> Prop :=
-| eq_syn_unit : eq_syn unit unit
-| eq_syn_send :
-    forall B S S',
-    eq_syn S S' ->
-    eq_syn (send B S) (send B S')
-| eq_syn_recv :
-    forall B S S',
-    eq_syn S S' ->
-    eq_syn (recv B S) (recv B S')
-| eq_syn_echoice :
-    forall S1 S2 S1' S2',
-    eq_syn S1 S1' ->
-    eq_syn S2 S2' ->
-    eq_syn (echoice S1 S2) (echoice S1' S2')
-| eq_syn_ichoice :
-    forall S1 S2 S1' S2',
-    eq_syn S1 S1' ->
-    eq_syn S2 S2' ->
-    eq_syn (ichoice S1 S2) (ichoice S1' S2')
-| eq_syn_mu :
-    forall xs xs' S S',
-    env_eq xs xs' ->
-    eq_syn S S' ->
-    eq_syn (mu xs S) (mu xs' S')
-| eq_syn_var :
-    forall X X',
-    X = X' ->
-    eq_syn (var X) (var X')
-.
-Hint Constructors eq_syn : styc.
-
-Local Hint Constructors eq_syn : tmp.
-Local Hint Resolve env_eq_refl env_eq_sym env_eq_trans : tmp.
-
-Lemma eq_syn_refl : reflexive Sty eq_syn.
-Proof. unfold reflexive. intros S. induction S; auto with tmp. Qed.
-
-Lemma eq_syn_sym : symmetric Sty eq_syn.
-Proof. unfold symmetric. intros S T HST. induction HST; auto with tmp. Qed.
-
-Lemma eq_syn_trans : transitive Sty eq_syn.
-Proof.
-  unfold transitive. intros S1 S2 S3 H12. generalize dependent S3. induction H12;
-  intros S3 H23; inversion_clear H23; subst; eauto with tmp.
-Qed.
-
-Add Relation Sty eq_syn
-  reflexivity proved by eq_syn_refl
-  symmetry proved by eq_syn_sym
-  transitivity proved by eq_syn_trans
-  as eq_syn'.
-
-Lemma eq_syn_shape :
-  forall S S',
-  eq_syn S S' ->
-  shape S = shape S'.
-Proof. intros S S' H. induction H; auto with styc. Qed.
-
-Hint Resolve eq_syn_shape : styc.
-
-Instance shape_m : Proper (eq_syn ==> eq) shape.
-Proof. unfold Proper. unfold respectful. apply eq_syn_shape. Qed.
 
 End StyC.
