ListAux.v
@@ -1,0 +1,14 @@
+Require Import List Logic.FunctionalExtensionality.
+Import ListNotations.
+
+Lemma fold_left_snoc :
+  forall A B (f : B -> A -> B) a0 x xs,
+  fold_left f (xs ++ [x]) a0 = f (fold_left f xs a0) x.
+Proof.
+  intros. rewrite <- fold_left_rev_right. rewrite rev_unit. simpl.
+  rewrite fold_left_rev_right.
+  assert ((fun x y => f x y) = f) as Hf.
+    apply functional_extensionality. intros.
+    apply functional_extensionality. auto.
+  rewrite Hf. trivial.
+Qed.
